{
 "cells": [
  {
   "cell_type": "markdown",
   "metadata": {},
   "source": [
    "# Homework 06\n",
    "\n",
    "In class, we discussed the L&L Example 6.4.1 growth model with and without an irreversible investment constraint: $f(k) \\geq c$.\n",
    "    \n",
    "$$\n",
    "\\max_{c(t)} \\int_0^T e^{-\\rho t} u(c(t)) dt \\qquad st \\qquad \\dot k = f(k) - c - mk\n",
    "$$\n",
    "\n",
    "Boundary conditions $k_0, k_T, T$\n",
    "\n",
    "Assume $u(c) = \\log c$ and $f(k) = k^\\alpha$\n",
    "\n",
    "Assume $\\alpha = 0.5, \\rho = 0.1, m = 0.3$.\n",
    "\n",
    "Have $k_0 = 1.15$ and $k_T = 0.6$ \n",
    "\n",
    "Need to get a couple of $T$ values\n",
    "\n",
    "# Solution\n",
    "\n",
    "The current value Hamiltonian and Lagrangian are\n",
    "$$\n",
    "\\tilde H(s,c,t) = u(c) + \\psi[f(k) - c - mk]\n",
    "$$\n",
    "\n",
    "$$\n",
    "\\mathcal L = u(c) + \\psi[f(k) - c - mk] + \\lambda[f(k) - c]\n",
    "$$\n",
    "\n",
    "The FONC are\n",
    "$$\n",
    "\\mathcal L_c = u'(c) - \\psi - \\lambda = 0\n",
    "$$\n",
    "The co-state is\n",
    "$$\n",
    "\\dot \\psi = [m+\\rho]\\psi -f'(k)[ \\psi + \\lambda]\n",
    "$$\n",
    "The state transition is\n",
    "$$\n",
    "\\dot k = [f(k) - c] - mk\n",
    "$$\n",
    "It'll be convenient to write that\n",
    "$$\n",
    "u'(c) = \\frac{1}{c} \\qquad \\qquad f'(k) = \\alpha k^{-(1-\\alpha)}\n",
    "$$"
   ]
  },
  {
   "cell_type": "markdown",
   "metadata": {},
   "source": [
    "## Unconstrained case\n",
    "\n",
    "In the unconstrained case, we have $\\lambda=0$, so\n",
    "$$\n",
    "u'(c) = \\psi \\qquad \\dot \\psi = [m+\\rho - f'(k)]\\psi \\qquad \\dot k = f(k) - c - mk\n",
    "$$\n",
    "Our convenient functional forms imply that $c = 1/\\psi$, so we can write these 2 ODEs as\n",
    "$$\n",
    "\\dot k = f(k) - 1/\\psi - mk \\qquad \\qquad \\dot \\psi = [m+\\rho - f'(k)]\\psi\n",
    "$$\n",
    "The interior nullclines are\n",
    "$$\n",
    "\\dot k \\geq 0 \\implies \\psi \\geq \\frac{1}{f(k)-mk} \\qquad \\qquad \\dot \\psi \\geq 0 \\implies k \\geq \\left(\\frac{\\alpha}{m+\\rho}\\right)^\\frac{1}{(1-\\alpha)}\n",
    "$$\n",
    "The steady state is where these hold with equality"
   ]
  },
  {
   "cell_type": "markdown",
   "metadata": {},
   "source": [
    "## Constrained case\n",
    "\n",
    "The constraint boundary is where $c \\geq f(k)$, which happens at $\\psi \\leq u'(f(k))$. At this point, we have that $\\psi + \\lambda = \\frac{1}{f(k)}$\n",
    "$$\n",
    "\\dot k = -mk \\qquad \\qquad \\dot \\psi = (m + \\rho)\\psi - \\frac{f'(k)}{f(k)} = (m+\\rho)\\psi - \\frac{\\alpha}{k}\n",
    "$$\n",
    "We have no constrained nullcline for $\\dot k$ as this would require $k=0$. For $\\psi$, we have that\n",
    "$$\n",
    "\\dot \\psi \\geq 0 \\implies \\psi \\geq \\frac{f'(k)}{(m+\\rho)c}\n",
    "$$"
   ]
  },
  {
   "cell_type": "markdown",
   "metadata": {},
   "source": [
    "We also need to figure out the value of entering in the second part of the problem. Once we enter the constrained region, we have that\n",
    "$$\n",
    "\\dot k = -mk \\implies k(t) = k_T e^{m(T-t)}\n",
    "$$\n",
    "Suppose the time the constraint binds is $\\hat t$. Then the integral is\n",
    "$$\n",
    "\\int_{\\hat t}^T e^{-\\rho t} \\log(k_T e^{m(T-t)}) dt\n",
    "$$\n",
    "We break this up into\n",
    "$$\n",
    "\\int_{\\hat t}^T e^{-\\rho t} \\log(k_T e^{m(T-t)}) dt = \\log(k_Te^{mT}) \\int_{\\hat t}^T e^{-\\rho t}dt - m \\int_{\\hat t}^T e^{-\\rho t} t dt\n",
    "$$\n",
    "The first piece is\n",
    "$$\n",
    "\\log(k_Te^{mT}) \\int_{\\hat t}^T e^{-\\rho t}dt = \\log(k_Te^{mT}) \\frac{e^{-\\rho \\hat t} - e^{-\\rho T}}{\\rho}\n",
    "$$\n",
    "The second piece we use [integration by parts](https://en.wikipedia.org/wiki/Integration_by_parts)\n",
    "$$\n",
    "\\int_a^b u(t)v'(t)dt = uv|_a^b - \\int_a^b u'(t)v(t)dt\n",
    "$$\n",
    "<!-- |_ asdf -->\n",
    "Take $u(t) = t$ and $v'(t) = e^{-\\rho t} \\implies v(t) = \\frac{e^{-\\rho t}}{-\\rho}$. Then\n",
    "$$\n",
    "\\int_{\\hat t}^T e^{-\\rho t} t dt = \\frac{e^{-\\rho \\hat t}(\\rho \\hat t + 1) - e^{-\\rho T}(\\rho T + 1)}{\\rho ^2} = \\frac{e^{-\\rho \\hat t}\\hat t - e^{-\\rho T} T}{\\rho} + \\frac{1}{\\rho}\\frac{e^{-\\rho \\hat t}- e^{-\\rho T}}{\\rho}\n",
    "$$\n",
    "Thus, we have that the current value of being at $t=\\hat t$ is this gross function:\n",
    "$$\n",
    "V(\\hat t; T, k_T) = \\int_{\\hat t}^T e^{-\\rho t} \\log(k_T e^{m(T-t)}) dt  = \\left[\\log(k_T e^{mT}) - \\frac m \\rho \\right]\\frac{e^{-\\rho \\hat t}- e^{-\\rho T}}{\\rho} - m\\frac{e^{-\\rho \\hat t}\\hat t - e^{-\\rho T} T}{\\rho}\n",
    "$$\n",
    "We need to be able to compute $\\frac{\\partial V}{\\partial \\hat t}$ ~~and $\\frac{\\partial V}{\\partial k(\\hat t)}$~~ to get our TVC right. We can get\n",
    "$$\n",
    "\\partial V / \\partial \\hat t = -\\left[\\log(k_T e^{mT}) - \\frac m \\rho \\right]e^{-\\rho \\hat t} + \\frac m \\rho e^{-\\rho \\hat t}\\left[\\rho \\hat t - 1\\right]\n",
    "$$\n",
    "~~We need $\\partial V / \\partial k_{\\hat t}$. First, we know that $k(\\hat t) = k_T e^{m(T-\\hat t)}$, so $k_Te^{mT} = \\hat k e^{m\\hat t}$~~\n",
    "$$\n",
    "\\partial V / \\partial \\hat k = \\frac{\\partial}{\\partial \\hat k} \\left\\{ \\left[\\log \\hat k + m\\hat t - \\frac m \\rho \\right]\\frac{e^{-\\rho \\hat t}- e^{-\\rho T}}{\\rho} - m\\frac{e^{-\\rho \\hat t}\\hat t - e^{-\\rho T} T}{\\rho} \\right\\} = \\frac{1}{\\hat k}\\frac{e^{-\\rho \\hat t}- e^{-\\rho T}}{\\rho}\n",
    "$$\n",
    "\n",
    "To pin down $\\hat t$, we write this as a free-end time problem for $\\hat t$ where we know $\\hat k = k_T e^{m(T-\\hat t)}$. The present value TVC given in L&L 7.6 (p 245) is\n",
    "$$\n",
    "H(s,c,\\pi,\\hat t) + \\frac{\\partial \\phi(b,\\hat t)}{\\partial \\hat t} = 0.\n",
    "$$\n",
    "For us, we'll have $\\phi(\\hat t) = e^{-\\rho \\hat t} V(\\hat t; T,k_T)$. So to convert this to current values, we multiply by $e^{\\rho \\hat t}$ and look at\n",
    "$$\n",
    "u(s,c) + \\psi f(s,c) + \\frac{ \\partial V(\\hat t;T,k_T)}{\\partial \\hat t} = 0\n",
    "$$\n",
    "Which gives us a nice root-finding problem in terms of $\\hat t$ given we have computed $\\hat k \\equiv k(\\hat t)$\n",
    "$$\n",
    "\\log f(\\hat k) + \\psi[-m \\hat k] - \\left[\\log(k_T e^{mT}) - \\frac m \\rho \\right]e^{-\\rho \\hat t} +  \\frac m \\rho e^{-\\rho \\hat t}\\left[\\rho \\hat t - 1\\right] = 0\n",
    "$$\n"
   ]
  },
  {
   "cell_type": "code",
   "execution_count": 5,
   "metadata": {},
   "outputs": [
    {
     "name": "stderr",
     "output_type": "stream",
     "text": [
      "┌ Info: Precompiling DifferentialEquations [0c46a032-eb83-5123-abaf-570d42b7fbaa]\n",
      "└ @ Base loading.jl:1242\n",
      "┌ Info: Recompiling stale cache file D:\\libraries\\julia\\compiled\\v1.2\\Plots\\ld3vC.ji for Plots [91a5bcdd-55d7-5caf-9e0b-520d859cae80]\n",
      "└ @ Base loading.jl:1240\n",
      "┌ Info: Recompiling stale cache file D:\\libraries\\julia\\compiled\\v1.2\\BasisMatrices\\65PSC.ji for BasisMatrices [08854c51-b66b-5062-a90d-8e7ae4547a49]\n",
      "└ @ Base loading.jl:1240\n"
     ]
    },
    {
     "ename": "ArgumentError",
     "evalue": "ArgumentError: Package ApproxFun not found in current path:\n- Run `import Pkg; Pkg.add(\"ApproxFun\")` to install the ApproxFun package.\n",
     "output_type": "error",
     "traceback": [
      "ArgumentError: Package ApproxFun not found in current path:\n- Run `import Pkg; Pkg.add(\"ApproxFun\")` to install the ApproxFun package.\n",
      "",
      "Stacktrace:",
      " [1] require(::Module, ::Symbol) at .\\loading.jl:876",
      " [2] top-level scope at In[5]:7"
     ]
    }
   ],
   "source": [
    "using DifferentialEquations\n",
    "using BoundaryValueDiffEq\n",
    "using Plots\n",
    "using Base: product\n",
    "using BasisMatrices\n",
    "using Optim\n",
    "using ApproxFun\n",
    "using LinearAlgebra: norm\n",
    "using NLsolve\n",
    "gr(fmt=:png)"
   ]
  },
  {
   "cell_type": "code",
   "execution_count": 3,
   "metadata": {},
   "outputs": [],
   "source": [
    "abstract type AbstractTVC end\n",
    "abstract type AbstractGrowthModel end\n",
    "\n",
    "struct TVC <: AbstractTVC\n",
    "    kstart::Float64\n",
    "    kstop::Float64\n",
    "    tmax::Float64\n",
    "end\n",
    "\n",
    "kstart(x::AbstractTVC) = x.kstart\n",
    "kstop(x::AbstractTVC) = x.kstop\n",
    "tmax(x::AbstractTVC) = x.tmax\n",
    "tmin(x::AbstractTVC) = zero(Float64)\n",
    "\n",
    "struct ConstrGrowthModel <: AbstractGrowthModel\n",
    "    alpha::Float64 # production\n",
    "    rho::Float64   # discount\n",
    "    depr::Float64  # depreciation\n",
    "end\n",
    "\n",
    "struct UnconstrGrowthModel <: AbstractGrowthModel\n",
    "    alpha::Float64 # production\n",
    "    rho::Float64   # discount\n",
    "    depr::Float64  # depreciation\n",
    "end\n",
    "\n",
    "# outer constructor\n",
    "(::AbstractGrowthModel)(;alpha=0.5, rho=0.1, depr=0.3) = (::AbstractGrowthModel)(alpha, rho, depr)\n",
    "\n",
    "const GrowthModel = AbstractGrowthModel\n",
    "\n",
    "#access fields of struct\n",
    "alpha(m::GrowthModel) = m.alpha\n",
    "rho(  m::GrowthModel) = m.rho\n",
    "depr( m::GrowthModel) = m.depr\n",
    "rho_depr(m::GrowthModel) = rho(m) + depr(m)\n",
    "\n",
    "# conversion\n",
    "ConstrGrowthModel(m::UnconstrGrowthModel) = ConstrGrowthModel(alpha(m), rho(m), depr(m))\n",
    "UnconstrGrowthModel(m::ConstrGrowthModel) = UnconstrGrowthModel(alpha(m), rho(m), depr(m))\n",
    "\n",
    "production(m::GrowthModel,k) = k^alpha(m)\n",
    "mglproduction(m::GrowthModel,k) = alpha(m)*k^(alpha(m)-1)\n",
    "utility(m::GrowthModel, c) = log(c)\n",
    "mglutility(m::GrowthModel, c) = 1/c\n",
    "\n",
    "# steady states\n",
    "function steady_state_k(m::GrowthModel)\n",
    "    frac = alpha(m)/rho_depr(m)\n",
    "    return frac^( 1/(1-alpha(m)) )\n",
    "end\n",
    "function steady_state_psi(m::GrowthModel)\n",
    "    khat = steady_state_k(m)\n",
    "    fk = production(m, khat)\n",
    "    return 1/(fk - depr(m)*khat)\n",
    "end\n",
    "steady_state(m::GrowthModel) = (steady_state_k(m), steady_state_psi(m),)\n",
    "\n",
    "# Value of being in constrained part\n",
    "function Vconstr(x::ConstrGrowthModel, tvc::AbstractTVC, that)\n",
    "    exp_rho_that = exp(-rho(x)*that)\n",
    "    exp_rho_T = exp(-rho(x)*tmax(tvc))\n",
    "    \n",
    "    a = log(kstop(tvc)) + depr(m)*tmax(tvc) - depr(x)/rho(x)\n",
    "    b = (exp_rho_that - exp_rho_T)/rho(x)\n",
    "    \n",
    "    c = depr(x)/rho(x)\n",
    "    d = exp_rho_that*that - exp_rho_T*tmax(tvc)\n",
    "    \n",
    "    return a*b - c*d\n",
    "end\n",
    "\n",
    "# Value of being in constrained part\n",
    "function dVconstr_dthat(x::ConstrGrowthModel, tvc::AbstractTVC, that)\n",
    "    exp_rho_that = exp(-rho(x)*that)   \n",
    "    a = log(kstop(tvc)) + depr(m)*tmax(tvc) - depr(x)/rho(x)\n",
    "    b = depr(x)/rho(x)*(rho(x)*that - 1)\n",
    "    return exp_rho_that*(-a + b)\n",
    "end\n",
    "\n",
    "\n",
    "# ODEs\n",
    "doti(m::UnconstrGrowthModel, k, i) = rho_delta(m) * (i - steady_state_i(m))\n",
    "dotk(m::InvestProb, k, i) = i - delta(m)*k\n",
    "\n",
    "# solvers in DifferentialEquations.jl require functions that\n",
    "# take the form   `f!(dy, y, params, t)`\n",
    "function dot_ki!(dy, y, m, t)\n",
    "    k,i = y\n",
    "    dy[1] = dotk(m, k, i)\n",
    "    dy[2] = doti(m, k, i)\n",
    "    return dy\n",
    "end"
   ]
  }
 ],
 "metadata": {
  "kernelspec": {
   "display_name": "Julia 1.2.0",
   "language": "julia",
   "name": "julia-1.2"
  },
  "language_info": {
   "file_extension": ".jl",
   "mimetype": "application/julia",
   "name": "julia",
   "version": "1.2.0"
  }
 },
 "nbformat": 4,
 "nbformat_minor": 4
}
